\newcommand{\naturals}{\mathbb N}

\paragraph{The \texttt{fftfreq} function}For \(n, N\in\naturals\),
\(0\leq n<N\), we introduce \(Z(n, N)\)
\begin{equation}
  Z(n, N)=
  \begin{cases}
    n & \text{if }2n<N,\\
    n-N & \text{otherwise.}
  \end{cases}
\end{equation}
For \(n<0\) or \(n\geq N\), \(Z(n, N)\) is defined by
\(N\)-periodicity. \(Z\) is very similar to the
\texttt{numpy.fft.fftfreq} function. Then
\begin{equation}
  Z(N-n, N)=
  \begin{cases}
    Z(n) & \text{if }2n=N,\\
    -Z(n) & \text{otherwise.}
  \end{cases}
\end{equation}
Indeed
\begin{enumerate}
\item If \(n=0\), then \(Z(N-n, N)=Z(N, N)=Z(0, N)=0=-Z(n, N)\).
\item If \(N\) is even, \(N=2M\)
  \begin{enumerate}
  \item If \(0<n<M\)
    \begin{gather*}
      2n<N\quad\Rightarrow\quad Z(n, N)=n,\\
      M<N-n\quad\Rightarrow\quad N<2\bigl(N-n\bigr)\quad\Rightarrow\quad Z(N-n, N)=N-n-N=-n.
    \end{gather*}
  \item If \(n=M\)
    \begin{gather*}
      2n=N\quad\Rightarrow\quad Z(n, N)=n-N=-M,\\
      2(N-n)=2M=N\quad\Rightarrow\quad Z(N-n, N)=-M.
    \end{gather*}
  \item If \(M<n<N\)
    \begin{gather*}
      N<2n\quad\Rightarrow\quad Z(n, N)=n-N,\\
     N-n<M\quad\Rightarrow\quad 2\bigl(N-n\bigr)<N\quad\Rightarrow\quad Z(N-n, N)=N-n.
    \end{gather*}
  \end{enumerate}
\item If \(N\) is odd, \(N=2M+1\)
  \begin{enumerate}
  \item If \(0<n\leq M\)
    \begin{gather*}
      2n\leq 2M<N\quad\Rightarrow\quad Z(n, N)=n,\\
      M+1\leq N-n\quad\Rightarrow\quad N<2\bigl(N-n\bigr)\quad\Rightarrow\quad Z(N-n, N)=N-n-N=-n.
    \end{gather*}
  \item If \(M+1\leq n<N\)
    \begin{gather*}
      N+1\leq 2n\quad\Rightarrow\quad Z(n, N)=n-N\\
      N-n\leq N-M-1=M\quad\Rightarrow\quad 2\bigl(N-n\bigr)\leq 2M<N\quad\Rightarrow\quad Z(N-n, N)=N-n
    \end{gather*}
  \end{enumerate}
\end{enumerate}
